SeqPL/Formula/Letterless.lean
@@ -1,0 +1,105 @@
+module
+
+public import SeqPL.Formula
+
+@[expose]
+public section
+
+namespace Formula
+
+abbrev Substitution (α) := α → Formula α
+
+@[grind]
+def subst (s : Substitution α) : Formula α → Formula α
+  | atom a  => (s a)
+  | ⊥       => ⊥
+  | □φ      => □(φ.subst s)
+  | φ 🡒 ψ   => φ.subst s 🡒 ψ.subst s
+notation:95 φ "⟦" s "⟧" => Formula.subst s φ
+
+variable {s : Substitution α} {A B : Formula α}
+
+lemma subst_atom : (#a)⟦s⟧ = s a := by grind;
+lemma subst_bot : (⊥)⟦s⟧ = ⊥ := by grind;
+lemma subst_top : (⊤)⟦s⟧ = ⊤ := by grind;
+lemma subst_imp : (A 🡒 B)⟦s⟧ = A⟦s⟧ 🡒 B⟦s⟧ := by rfl
+lemma subst_and : (A ⋏ B)⟦s⟧ = A⟦s⟧ ⋏ B⟦s⟧ := by grind;
+lemma subst_or  : (A ⋎ B)⟦s⟧ = A⟦s⟧ ⋎ B⟦s⟧ := by grind;
+lemma subst_neg : (∼A)⟦s⟧ = ∼(A⟦s⟧) := by grind;
+lemma subst_iff : (A 🡘 B)⟦s⟧ = A⟦s⟧ 🡘 B⟦s⟧ := by grind;
+attribute [simp, grind =]
+  subst_atom
+  subst_bot
+  subst_top
+  subst_neg
+  subst_and
+  subst_or
+  subst_imp
+  subst_iff
+@[simp, grind =] lemma subst_box : (□A)⟦s⟧ = □(A⟦s⟧) := by grind;
+@[simp, grind =] lemma subst_boxItr {n : ℕ} : (□^[n]A)⟦s⟧ = □^[n](A⟦s⟧) := by induction n generalizing A <;> grind;
+@[simp, grind =] lemma subst_dia : (◇A)⟦s⟧ = ◇(A⟦s⟧) := by grind;
+@[simp, grind =] lemma subst_diaItr {n : ℕ} : (◇^[n]A)⟦s⟧ = ◇^[n](A⟦s⟧) := by induction n generalizing A <;> grind;
+
+end Formula
+
+
+variable {α : Type*}
+
+abbrev LetterlessFormula := Formula Empty
+
+namespace LetterlessFormula
+
+variable {A : LetterlessFormula}
+
+def lift : LetterlessFormula → Formula α
+  | ⊥ => ⊥
+  | A 🡒 B => lift A 🡒 lift B
+  | □A => □(lift A)
+instance : Coe LetterlessFormula (Formula α) := ⟨lift⟩
+
+@[simp, grind =] lemma eq_subst_self : A⟦s⟧ = A := by induction A <;> grind;
+
+end LetterlessFormula
+
+
+abbrev LetterlessFormulaList := FormulaList Empty
+
+abbrev LetterlessFormulaFinset := FormulaFinset Empty
+
+namespace LetterlessFormulaFinset
+
+def lift [DecidableEq α] : LetterlessFormulaFinset → FormulaFinset α := λ Γ => Γ.image (LetterlessFormula.lift)
+instance [DecidableEq α] : Coe LetterlessFormulaFinset (FormulaFinset α) := ⟨lift⟩
+
+end LetterlessFormulaFinset
+
+
+abbrev LetterlessFormulaSet := FormulaSet Empty
+
+namespace LetterlessFormulaSet
+
+def lift : LetterlessFormulaSet → FormulaSet α := λ Γ => Γ.image (LetterlessFormula.lift)
+instance : Coe LetterlessFormulaSet (FormulaSet α) := ⟨lift⟩
+
+end LetterlessFormulaSet
+
+
+namespace Formula
+
+def Letterless : Formula α → Prop
+  | #_ => False
+  | ⊥ => True
+  | A 🡒 B => A.Letterless ∧ B.Letterless
+  | □A => A.Letterless
+
+def toLetterless : (A : Formula α) → (_ : Letterless A) → LetterlessFormula
+  | ⊥, _ => ⊥
+  | A 🡒 B, ⟨hA, hB⟩ => toLetterless A hA 🡒 toLetterless B hB
+  | □A, hA => □(toLetterless A hA)
+
+end Formula
+
+
+
+end
