SeqPL/Logic/SumQuasiNormal.lean
@@ -1,0 +1,48 @@
+module
+
+public import SeqPL.Logic.Basic
+public import SeqPL.Formula.Letterless
+
+@[expose]
+public section
+
+@[grind]
+inductive Logic.sumQuasiNormal (L₁ L₂ : Logic α) : Logic α
+  | mem₁ {A}    : L₁ A → sumQuasiNormal L₁ L₂ A
+  | mem₂ {A}    : L₂ A → sumQuasiNormal L₁ L₂ A
+  | mdp  {A B}  : sumQuasiNormal L₁ L₂ (A 🡒 B) → sumQuasiNormal L₁ L₂ A → sumQuasiNormal L₁ L₂ B
+  | subst {A s} : sumQuasiNormal L₁ L₂ A → sumQuasiNormal L₁ L₂ (A⟦s⟧)
+infix:50 " +ᴸ " => Logic.sumQuasiNormal
+
+namespace Logic.sumQuasiNormal
+
+variable {L₁ L₂ : Logic α} {A B : Formula α} {s : Formula.Substitution α}
+
+@[grind .] lemma subset_L₁ : L₁ ⊆ (L₁ +ᴸ L₂) := by apply Logic.sumQuasiNormal.mem₁;
+@[grind .] lemma subset_L₂ : L₂ ⊆ (L₁ +ᴸ L₂) := by apply Logic.sumQuasiNormal.mem₂;
+
+end Logic.sumQuasiNormal
+
+
+abbrev Logic.addQuasiNormal (L : Logic α) (A : Formula α) := L +ᴸ {A}
+infixl:50 " +ᴸ " => Logic.addQuasiNormal
+
+
+abbrev LogicS (α) := (LogicGL α) +ᴸ ({ □A 🡒 A | A })
+
+abbrev LogicD (α) := (LogicGL α) +ᴸ (insert (∼□⊥) { □(□A ⋎ □B) 🡒 (□A ⋎ □B) | (A) (B) })
+
+lemma LogicS_subset_LogicD : LogicD α ⊆ LogicS α := by
+  intro A h;
+  induction h with
+  | mem₁ h => apply Logic.sumQuasiNormal.mem₁; exact h
+  | mdp h₁ h₂ ih₁ ih₂ => apply Logic.sumQuasiNormal.mdp; exact ih₁; exact ih₂
+  | subst h ih => apply Logic.sumQuasiNormal.subst; exact ih
+  | mem₂ h =>
+    rcases h with (rfl | ⟨A, B, rfl⟩);
+    . apply Logic.sumQuasiNormal.mem₂;
+      use ⊥;
+    . apply Logic.sumQuasiNormal.mem₂;
+      use (□A ⋎ □B);
+
+end
